current-formalism/Gathering/InR2/Algorithm.v
@@ -656,25 +656,63 @@ Proof.
 Qed.
 
 
-Lemma R2middle_morph : forall x y (sim:Sim.t), (R2.middle (sim x) (sim y))%R2 = sim ((R2.middle x y))%R2.
-  Proof.
-  (*   intros x y sim.     *)
-  (*   unfold R2.middle. *)
-  (*   assert (hrinv:(Rinv 2 = Rdiv 1 2)%R). *)
-  (*   { field_simplify.  reflexivity. } *)
-  (*   setoid_rewrite <- hrinv. *)
-  (*   setoid_rewrite <- middle_is_barycenter_3. *)
-  (*   apply barycenter_morph. *)
-  (* unfold R2.middle. *)
-  (* assert (Rinv 2 = Rdiv 1 2)%R. *)
-  (* { field_simplify.  reflexivity. } *)
-  (* rewrite ?H0 in *. *)
-  (* rewrite <- H. *)
-  (* rewrite <- barycenter_morph. *)
-  (* assert ((/ 2 * (x + y))%R2 = (1 / 2 * (x + y))%R2). *)
-  (* destruct x, y;cbn. *)
+Lemma R2_is_middle_morph : forall x y C (sim:Sim.t), is_middle x y C -> (is_middle (sim x) (sim y) (sim C)).
+Proof.
+  intros x y C sim hmid.
+  red.
+  intros p.
+  unfold is_middle in hmid.
+  rewrite <- (@Similarity.section_retraction _ _ _ (sim.(Sim.sim_f)) p).
+  setoid_rewrite sim.(Sim.dist_prop).
+  setoid_rewrite R_sqr.Rsqr_mult.
+  setoid_rewrite <- Rmult_plus_distr_l.
+  apply Rmult_le_compat_l.
+  - apply Rle_0_sqr.
+  - apply hmid.
+Qed.
 
-Admitted.
+
+Lemma R2_middle_morph : forall x y (sim:Sim.t), (R2.middle (sim x) (sim y))%R2 = sim ((R2.middle x y))%R2.
+Proof.
+  intros x y sim.
+  generalize (@middle_spec x y).
+  intro hmidlxy.
+  generalize (@middle_spec (sim x) (sim y)).
+  intro hmidsimxy.
+  assert (is_middle (sim x) (sim y) (sim (R2.middle x y))).
+  { apply R2_is_middle_morph.
+    auto. }
+  apply middle_unique with (sim x) (sim y);assumption.
+Qed.
+
+Lemma R2_is_bary3_morph : forall x y z C (sim:Sim.t), is_barycenter_3_pt x y z C -> (is_barycenter_3_pt (sim x) (sim y) (sim z) (sim C)).
+Proof.
+  intros x y z C sim hmid.
+  red.
+  intros p.
+  unfold is_barycenter_3_pt in hmid.
+  rewrite <- (@Similarity.section_retraction _ _ _ (sim.(Sim.sim_f)) p).
+  setoid_rewrite sim.(Sim.dist_prop).
+  setoid_rewrite R_sqr.Rsqr_mult.
+  repeat setoid_rewrite <- Rmult_plus_distr_l.
+  apply Rmult_le_compat_l.
+  - apply Rle_0_sqr.
+  - apply hmid.
+Qed.
+
+
+Lemma R2_bary3_morph : forall x y z (sim:Sim.t), (barycenter_3_pts (sim x) (sim y) (sim z))%R2 = sim ((barycenter_3_pts x y z))%R2.
+Proof.
+  intros x y z sim.
+  generalize (@bary3_spec x y z).
+  intro hmidlxy.
+  generalize (@bary3_spec (sim x) (sim y) (sim z)).
+  intro hmidsimxy.
+  assert (is_barycenter_3_pt (sim x) (sim y) (sim z) (sim (barycenter_3_pts x y z))).
+  { apply R2_is_bary3_morph.
+    auto. }
+  apply bary3_unique with (sim x) (sim y) (sim z);assumption.
+Qed.
 
 
 Lemma target_morph : forall (sim : Sim.t) s,target (Spect.map sim s) = sim (target s).
